[224. Basic Calculator](https://leetcode.com/problems/basic-calculator/)

* Amazon, Facebook, Indeed, Karat, Roblox, Google, Microsoft, Robinhood
* Math, Stack
* Similar Questions:
    * Evaluate Reverse Polish Notation
    * [227. Basic Calculator II](https://leetcode.com/problems/basic-calculator-ii/)
    * Different Ways to add Parentheses
    * Expression Add Operations
    * [772. Basic Calculator III](https://leetcode.com/problems/basic-calculator-iii/)


[Java - Common template for Basic Calculator I, II, and III using Stack](https://leetcode.com/problems/basic-calculator-iii/discuss/344371/Java-Common-template-for-Basic-Calculator-I-II-and-III-using-Stack)



## Analysis

* Input always contains valid strings.
* The rules of addition and substraction.
* Implication of precedence by parenthesis. [括号隐含的优先级信息]
* Spaces do not affect the evaluation of the input expression.

We push the elements of the expression one by one onto the stack until we get a closing bracket `)`. Then we pop the elements from the stack one by one and evaluate the expression on-the-go. This is done till we find the corresponding opening bracket `(`.



## Method 1. Common Template (Slow)

Key Points:

1. Use `-` operator as the magnitude for the operand to the right of the operator, for e.g. `A - B - C` could be re-written as `A + (-B) + (-C)`. **The re-written expression would follow associativity rule. Thus evaluating the expression from right or left, won't change the result.**
2. What we need to keep in mind is that the expression given would be complicated, i.e. there would be expressions nested within other expressions.

**Intuition:** 
* Associate the sign with the expression to the **right** of it. 
* `+,-,)` mark the end of an operand. Thus this is the right time we can use this operand and this sign to the left of the operand for evaluation.

```java 
class Solution {
    public int calculate(String s) {
        if(s == null || s.length() == 0) {
            return 0;
        }
        
        Stack<Integer> stack = new Stack<Integer>();
        int num = 0;        // Represent current value, like 123 in `234 + 123`
        char sign = '+';    // The initial sign for the first num, like `+` of 234
        char[] ss = s.toCharArray();
        
        for(int i=0; i<ss.length; i++) {
            if(Character.isDigit(ss[i])) {
                num = 10 * num + (ss[i] - '0');
            } else if(ss[i] == '(') {
                int cnt = 0;    // the num of braces, cnt=0 means there is a valid pair
                int j = i;
                for( ; i<ss.length; i++) {
                    if(ss[i] == '(') {
                        cnt++;
                    } else if(ss[i] == ')') {
                        cnt--;
                    }
                    if(cnt == 0) {
                        break;
                    }
                }   // When breaking out of this loop, ss[i]==')'
                num = calculate(s.substring(j+1, i));   // s[j+1, i)
            }
            
            if(ss[i]=='+' || ss[i]=='-' || i==ss.length-1) {    // i==ss.length-1, make sure the last num is added to the stack
                switch(sign) {
                    case '+':
                        stack.push(num);
                        break;
                    case '-':
                        stack.push(-num);
                        break;
                }
                num = 0;
                sign = ss[i];
            }
        }
        int res = 0;
        while(!stack.isEmpty()) {
            res += stack.pop();
        }
        return res;
    }
}
```



## Method 2. Array (Without Stack)

* 相当与每个数字都有一个符号，默认的 `sign = 1` 说明第一个 number 的符号是 `+`；
* 遇到一个符号的时候，就将之前的数字和符号合并到一起，i.e. `res += sign * num` and set `num = 0`;
* '(': Need recall this function on rest sub-string;
* ')': Need update pos[0] and return res.
* The character will face:
    * ' '
    * digit: [0,9]
    * sign: + - * /
    * (
    * )
* 遇到新的符号或是到字符串结尾的时候，对最新的 `num` 进行处理。
```java 
class Solution {
    public int calculate(String s) {
        if(s==null || s.length()==0) {
            return 0;
        }
        return calculate(s.toCharArray(), new int[]{0});
    }
    
    private int calculate(char[] s, int[] pos) {
        int res = 0;
        int num = 0;
        int sign = 1;
        int i = pos[0]; // index iterate through the char array s
        
        while(i < s.length) {
            switch(s[i]) {
                case ' ':
                    break;
                case '+':
                    sign = 1;
                    break;
                case '-':
                    sign = -1;
                    break;
                case '(':	// calcuate sub-expression
                    pos[0] = i + 1;
                    res += sign * calculate(s, pos);
                    i = pos[0]; // s[i] == ')'
                    break;
                case ')':
                    pos[0] = i;
                    return res + sign * num;
                default:
                    num = 10 * num + (s[i] - '0');
                    // When the next character is not a digit, then update res and reset num
                    if(i+1==s.length || !Character.isDigit(s[i+1])) {
                        res += sign * num;
                        num = 0;
                    }
            }
            i++;
        }
        return res + sign * num;
    }
}
```



## Method 3. Stack and String Reversal
> This question qualifies really well for a stack question. 
> **Since the expression might have parentheses, we can use a stack to find the value for each sub-expression within a parenthesis.**
> 
> We push the elements of the expression one by one onto the stack until we get a closing bracket `)`.
> Then we pop the elements from the stack one by one and evaluate the expression on-the-go. This is done till we find the corresponding `(` opening bracket.
> 1. 将element一个一个push进Stack，直到遇到`)`，然后开始从stack中pop元素，开始处理expression。
> 2. 直到遇到`(`，说明一个sub-expression结束了。

**Note:**
If we use a stack and read the elements of the expression from left to right, we end up evaluating the expression from right-to-left. This means we are expecting `(A−B)−C` to be equal to `(C−B)−A` which is not correct. Subtraction is neither associative nor commutative.(减法既不结合也不满足交换律。)
This problem could be solved very easily by reversing the string and then using basic drill using a stack.

```java 
class Solution {
    public int calculate(String s) {
        Stack<Integer> stack = new Stack<Integer>();
        int operand = 0;
        int res = 0;    // For the on-going result
        int sign = 1;   // 1 means positive, and -1 means negative
        
        for(int i=0; i<s.length(); i++) {
            char ch = s.charAt(i);
            
            switch(ch) {
                case ' ':
                    break;
                case '+':
                    // Evaluate the expression to the left with result, sign and operand
                    res += sign * operand;
                    sign = 1;       // Save the recently encounted '+' sign
                    operand = 0;    // Reset operand
                    break;
                case '-':
                    res += sign * operand;
                    sign = -1;
                    operand = 0;
                    break;
                case '(':
                    // Push the result and sign onto the stack,
                    // for later we push result first, then sign
                    stack.push(res);    // res before this '('
                    stack.push(sign);   // the last sign before this '('
                    // Reset operand and result, as if new evaluate begins for the new sub-expression
                    sign = 1;
                    res = 0;
                    break;
                case ')':
                    // Evaluate the expression to the left with result, sign and operand
                    res += sign * operand;
                    // ')' marks the end of expression within a set of parenthesis.
                    // Its result is multiplied with sign on top of stack as stack.pop() is the sign before the parenthesis
                    res *= stack.pop();
                    // Then add to the next operand on the top,
                    // as stack.pop() is the result calculated before this parenthesis
                    // (operand on stack) + (sign on stack * (res from parenthesis))
                    res += stack.pop();
                    // Reset the operand
                    operand = 0;
                    break;
                default:
                    operand = 10 * operand + (ch - '0');
            }
        }
        return res + sign * operand;
    }
}
```
**Complexity Analysis:**
1. Time Complexity: `O(N)`, where `N` is the length of the string. The difference in time complexity between this approach and the previous one is that every character in this approach will get processed exactly once. 
However, in the previous approach, each character can potentially get processed twice, once when it's pushed onto the stack and once when it's popped for processing of the final result (or a subexpression). That's why this approach is faster.
2. Space Complexity: `O(N)`, where `N` is the length of the string. 

### 变体
```Java
class Solution {
    public int calculate(String s) {
        Deque<Integer> stack = new ArrayDeque<>();
        
        int res = 0;
        int sign = 1;
        int currNum = 0;
        for(int i=0; i<s.length(); i++) {
            char c = s.charAt(i);

            if(Character.isDigit(c)) {
                currNum = currNum * 10 + (c - '0');
            }
            if(c == '+' || c == '-') {
                res += sign * currNum;
                sign = (c == '+') ? 1 : -1;
                currNum = 0;
            } else if(c == '(') {
                stack.push(res);
                stack.push(sign);
                sign = 1;
                res = 0;
            } else if(c == ')') {
                res += sign * currNum;
                res *= stack.pop();
                res += stack.pop();
                currNum = 0;
            }
        }
        return res + sign * currNum;
    }
}  
```


## Method 3. Stack + without reverse
```Java
class Solution {
    public int calculate(String s) {
        Deque<Integer> stack = new ArrayDeque<>();
        int result = 0; // For the on-going result
        int operand = 0;
        int sign = 1;   // 1 means positive, -1 means negative
        for(int i=0; i<s.length(); i++) {
            char ch = s.charAt(i);
            if(Character.isDigit(ch)) {
                operand = operand * 10 + (ch - '0');
            } else if(ch == '+') {
                result += sign * operand;
                sign = 1;
                operand = 0;
            } else if(ch == '-') {
                result += sign * operand;
                sign = -1;
                operand = 0;
            } else if(ch == '(') {
                stack.push(result);
                stack.push(sign);
                sign = 1;
                result = 0;
            } else if(ch == ')') {
                result += sign * operand;
                result *= stack.pop();
                result += stack.pop();
                operand = 0;
            }
        }
        return result + (sign * operand);
    }
}
```
**Complexity Analysis:**
1. Time Complexity: `O(N)`, where `N` is the length of the string. The difference in time complexity between this approach and the previous one is that every character in this approach will get processed exactly once. However, in the previous approach, each character can potentially get processed twice, once when it's pushed onto the stack and once when it's popped for processing of the final result (or a subexpression). That's why this approach is faster.
2. Space Complexity: `O(N)`, where N is the length of the string.


## Reference
* https://leetcode.com/problems/basic-calculator-ii/editorial/